Modification on AbstractMultiPaxosR1.thy

Isabelle2/BallotArrays.thy
@@ -1,45 +1,42 @@
 section {* Definition of ballot arrays *}
 
 theory BallotArrays
-imports Main LinorderOption
+imports Main "~~/src/HOL/Library/Monad_Syntax" LinorderOption Quorums Max_Properties
 begin
 
+subsection {* The definitions *}
+
 locale ballot_array =
-  -- {* @{typ 'a} is the type of acceptors *}
-  fixes ballot :: "'a \<Rightarrow> nat"
-  and vote :: "'a \<Rightarrow> nat \<Rightarrow> 'v option"
-  and quorums :: "'a set set"
+  fixes quorums :: "'a set set"
+  and ballot :: "'a \<Rightarrow> nat"
+  and vote :: "'a \<Rightarrow> nat \<rightharpoonup> 'v"
 begin
 
 definition conservative where
   "conservative b \<equiv> \<forall> a1 . \<forall> a2 .
-    let v1 = vote a1 b; v2 = vote a2 b in 
+    let v1 = vote a1 b; v2 = vote a2 b in
       case v1 of Some x \<Rightarrow> (case v2 of Some y \<Rightarrow> x = y | None \<Rightarrow> True) | None \<Rightarrow> True"
 
 definition conservative_array where
   "conservative_array \<equiv> \<forall> b . conservative b"
 
 text {* Here the @{term Max} is the one from @{text Lattices_Big} *}
-    
-definition max_voted_round_q where
-  "max_voted_round_q q bound \<equiv> 
-    if \<exists> b a . a \<in> q \<and> b \<le> bound \<and> vote a b \<noteq> None
-    then Some (Max {b . \<exists> a . a \<in> q \<and> b \<le> bound \<and> vote a b \<noteq> None})
-    else None"
- 
-definition is_safe where
-  "is_safe q bound v \<equiv>
-    case max_voted_round_q q bound of
-      None \<Rightarrow> True
-    | Some b \<Rightarrow> \<exists> a . a \<in> q \<and> vote a b = Some v"
 
-definition proved_safe_at where
-  "proved_safe_at Q b v \<equiv>
-    case b of 0 \<Rightarrow> True
-    | Suc c \<Rightarrow> Q \<in> quorums \<and> (\<forall> a \<in> Q . ballot a \<ge> b) \<and> is_safe Q c v"
+definition proved_safe_at_2_a where
+  "proved_safe_at_2_a q b v \<equiv>
+    q \<in> quorums \<and> (\<forall> a \<in> q . ballot a \<ge> b) \<and>
+    (if \<exists> a \<in> q . \<exists> b\<^sub>2 . b\<^sub>2 < b \<and> vote a b\<^sub>2 \<noteq> None
+    then \<exists> a \<in> q . vote a (Max {b\<^sub>2 . \<exists> a \<in> q . b\<^sub>2 < b \<and> vote a b\<^sub>2 \<noteq> None}) = Some v
+    else True)"
+
+definition voted_bal where
+  "voted_bal a v_bal b \<equiv> v_bal < b \<and> vote a v_bal \<noteq> None"
+
+lemma finite_voted_bal:"finite {b\<^sub>a. voted_bal a b\<^sub>a b}"
+by (simp add: voted_bal_def)
 
 definition chosen_at where
-  "chosen_at v b \<equiv> \<exists> q . q \<in> quorums \<and> (\<forall> a \<in> q . (vote) a b = (Some v))"
+  "chosen_at v b \<equiv> \<exists> q . q \<in> quorums \<and> (\<forall> a \<in> q . vote a b = (Some v))"
 
 definition chosen where
   "chosen v \<equiv> \<exists> b . chosen_at v b"
